{
 "cells": [
  {
   "cell_type": "markdown",
   "metadata": {},
   "source": [
    "\\begin{array}{|c|c|c|c|c|}\n",
    "  \\hline\n",
    "  r.v. & \\text{Probability Mass Function} & \\text{Mean} & \\text{Variance} & \\text{Moment Generating Function}\\\\\n",
    "  \\hline\n",
    "\\text{Uniform}&\\frac{1}{b-a+1} & \\frac{a+b}{2} & \\frac{(b-a+1)^2-1}{12} & \\frac{e^{a t}-e^{(b+1) t}}{(b-a+1)(1-e^t)}  \\\\\\hline\n",
    "\\text{Bernoulli} &p^x(1-p)^{1-x},x=0,1&p&p(1-p)&(1-p)+pe^t\\\\\\hline\n",
    "\\text{Binomial}&C^n_k p^k(1-p)^{n-k}&np&np(1-p)&((1-p)+pe^t)^n\\\\\\hline\n",
    "\\text{Geometric}&p(1-p)^{k}&(1-p)/p&(1-p)/p^2&\\frac{p}{1-(1-p)e^t}\\\\\\hline\n",
    "\\text{negativeBinom}&C^{k+r-1}_k(1-p)^kp^r&\\frac{r(1-p)}{p}&\\frac{r(1-p)}{p^2}&\\left(\\frac{p}{1-(1-p)e^t}\\right)^r\\\\\\hline\n",
    "\\text{Poisson}&\\frac{e^{-\\lambda}\\lambda^x}{x!}&\\lambda&\\lambda&e^{\\lambda(e^t-1)}\\\\\\hline\n",
    "\\end{array}\n"
   ]
  },
  {
   "cell_type": "markdown",
   "metadata": {},
   "source": [
    "D-Uniform\n",
    "---\n",
    "1. $X=a,a+1,a+2,\\cdots,b-1,b$, where $b>a$ and $a,b\\in\\mathbb Z$;\n",
    "- pmf: $f_X(x)=\\frac{1}{b-a+1}$\n",
    "- Mean: \n",
    "   $$EX=\\sum_{x=a}^{b}x P(X=x)=\\sum_{x=a}^{b}\\frac{x}{b-a+1}=\\frac{1}{b-a+1}\\sum_{x=a}^{b}{x}=\\frac{a+b}{2}$$\n",
    "- Variance;\n",
    "\\begin{eqnarray}\n",
    " Var(X)&=&E(X-\\mu)^2=E\\left((X-a)-(\\mu-a)\\right)^2\\\\\n",
    "   &=& E(X-a)^2-(\\mu-a)^2\\\\   \n",
    "   &=&\\sum_{x=a}^{b}(x-a)^2 P(X=x)-\\left(\\frac{b-a}{2}\\right)^2\\\\\n",
    "   &=&\\frac{\\sum\\limits_{x=0}^{b-a}x^2}{b-a+1}-\\frac{(b-a)^2}{4}\\\\\n",
    "   &=&\\frac{(b-a)(b-a+1)(2b-2a+1)}{6(b-a+1)}-\\frac{(b-a)^2}{4}\\\\\n",
    "   &=&\\frac{(b-a)(b-a+2)}{12}=\\frac{(b-a+1)^2-1}{12}\n",
    "\\end{eqnarray}\n",
    "Note that $X-a=0,1,2,\\cdots,b-a)$.\n",
    "- MGF:\n",
    "\\begin{eqnarray}\n",
    " E e^{tX}&=&\\sum_{x=a}^{b}e^{tx} P(X=x)\\\\\n",
    "         &=&\\frac{\\sum_{x=a}^{b}e^{tx}}{b-a+1}=\\frac{e^{at}}{b-a+1}(1+e^t+e^{2t}+\\cdots+e^{(b-a)t})\\\\\n",
    "         &=&\\frac{e^{at}(1-e^{(b-a+1)t})}{(b-a+1)(1-e^t)}= \\frac{e^{a t}-e^{(b+1) t}}{(b-a+1)(1-e^t)}\n",
    "\\end{eqnarray}"
   ]
  },
  {
   "cell_type": "markdown",
   "metadata": {},
   "source": [
    "Bernoulli\n",
    "---\n",
    "1. $X=0,1$ with pmf: $p^x(1-p)^{1-x},x=0,1$;\n",
    "- Mean: \n",
    "   $$EX=\\sum_{x=a}^{b}x P(X=x)=0\\cdot(1-p)+1\\cdot p=p$$\n",
    "- Variance;\n",
    "\\begin{eqnarray}\n",
    " Var(X)&=&E X^2 - \\mu^2=0^2\\cdot(1-p)+1^2\\cdot p-p^2=p(1-p)\n",
    "\\end{eqnarray}\n",
    "- MGF:\n",
    "\\begin{eqnarray}\n",
    "   E e^{tX}&=&e^0\\cdot (1-p) +e^t\\cdot p=1-p+pe^t\\\\\n",
    "\\end{eqnarray}"
   ]
  },
  {
   "cell_type": "markdown",
   "metadata": {},
   "source": [
    "Binomial\n",
    "---\n",
    "1. Let $X_1,X_2,\\cdots X_n$ be i.i.d. of Bernoulli, $X=0,1$ with pmf: $p^x(1-p)^{1-x},x=0,1$; then $Y=\\sum_{i=1}^n X_i$ is Binomial;\n",
    "- Mean: \n",
    "   $$EY=E\\left(\\sum_iX_i\\right)=\\sum_iEX_i=n\\cdot p$$\n",
    "- Variance;\n",
    "\\begin{eqnarray}\n",
    " Var(Y)&=&\\sum_i E X_i^2 =n\\cdot p(1-p)\n",
    "\\end{eqnarray}\n",
    "since i.i.d;\n",
    "- MGF:\n",
    "\\begin{eqnarray}\n",
    "   E e^{tY}&=&Ee^{tY}=Ee^{\\sum_i tX_i}=\\prod_iEe^{tX_i}=(1-p+pe^t)^n\\\\\n",
    "\\end{eqnarray}"
   ]
  },
  {
   "cell_type": "markdown",
   "metadata": {},
   "source": [
    "Geometric\n",
    "---\n",
    "1. $X$'s pmf: $f_X(X=k)=p(1-p)^{k},k=0,1,2,3,4,\\cdots$;\n",
    "- MGF:\n",
    "\\begin{eqnarray}\n",
    "   M_X(t)=E e^{tX}&=&\\sum_{k=0}^\\infty e^{tk}p(1-p)^{k}=\\sum_{k=0}^\\infty p\\left((1-p)e^t\\right)^k=\\frac{p}{1-(1-p)e^t}\\\\\n",
    "\\end{eqnarray}\n",
    "- Mean: \n",
    "\\begin{eqnarray}\n",
    "   EX &=&M_X'(0)=(Ee^{tX})'=\\left.EXe^{tX}\\right|_{t=0}=EX\\\\\n",
    "   &=& \\left(\\frac{p}{1-(1-p)e^t}\\right)'\\\\\n",
    "   &=& \\left.\\frac{p}{(1-(1-p)e^t)^2}\\cdot((1-p)e^t)\\right|_{t=0}\n",
    "   &=& \\frac{1-p}{p}\n",
    "\\end{eqnarray}   \n",
    "- Variance;  similar as above:\n",
    "\\begin{eqnarray}\n",
    " Var(X)&=&E X^2 - \\mu^2= M_X''(0)-\\left(\\frac{1-p}{p}\\right)^2\\\\\n",
    "  &=& \\left.\\left[\\frac{2p}{(1-(1-p)e^t)^3}\\cdot((1-p)e^t)^2+\\frac{p}{(1-(1-p)e^t)^2}\\cdot((1-p)e^t)\\right]\\right|_{t=0}-\\left(\\frac{1-p}{p}\\right)^2\\\\\n",
    "  &=&\\frac{2p(1-p)^2}{p^3}+\\frac{(1-p)}{p}-\\left(\\frac{1-p}{p}\\right)^2\n",
    "   =\\frac{1-p}{p^2}\n",
    "\\end{eqnarray}\n"
   ]
  },
  {
   "cell_type": "markdown",
   "metadata": {},
   "source": [
    "Negative Binomial\n",
    "---\n",
    "1. Let $Y=\\sum_{i=1}^rX_i$ where $\\{X_i\\}$ are i.i.d of $X$, geometric r.v.;\n",
    "- Mean: \n",
    "   $$EY=E\\left(\\sum_iX_i\\right)=\\sum_iEX_i=\\frac{r(1-p)}{p}$$\n",
    "- Variance;\n",
    "\\begin{eqnarray}\n",
    " Var(Y)&=&\\sum_i E X_i^2 =\\frac{r(1-p)}{p^2}\n",
    "\\end{eqnarray}\n",
    "since i.i.d;\n",
    "- MGF:\n",
    "\\begin{eqnarray}\n",
    "   E e^{tY}&=&Ee^{tY}=Ee^{\\sum_i tX_i}=\n",
    "   \\prod_i Ee^{tX_i}=\\left(\\frac{p}{1-(1-p)e^t}\\right)^r\\\\\n",
    "\\end{eqnarray}"
   ]
  },
  {
   "cell_type": "markdown",
   "metadata": {},
   "source": [
    "Poisson\n",
    "---\n",
    "1. $X$'s pmf: $f_X(X=x)=\\frac{e^{-\\lambda}\\lambda^x}{x!},x=0,1,2,3,\\cdots$;\n",
    "- MGF:\n",
    "\\begin{eqnarray}\n",
    "   M_X(t)=E e^{tX}&=&\\sum_{x=0}^\\infty e^{tx}\\frac{e^{-\\lambda}\\lambda^x}{x!}=e^{-\\lambda}\\sum_{x=0}^\\infty \\frac{(\\lambda e^t)^x}{x!}=e^{-\\lambda}e^{\\lambda e^t}\n",
    "   =e^{\\lambda(e^t-1)}\\\\\n",
    "\\end{eqnarray}\n",
    "by the fact of \n",
    "$$e^x=\\sum_{n=0}^\\infty=\\frac{x^n}{n!}$$\n",
    "- Mean: \n",
    "\\begin{eqnarray}\n",
    "   EX &=&M_X'(0)=(Ee^{tX})'=\\left.EXe^{tX}\\right|_{t=0}=EX\\\\\n",
    "   &=& \\left.\\lambda e^te^{\\lambda(e^t-1)} )\\right|_{t=0}=\\lambda\n",
    "\\end{eqnarray}   \n",
    "- Variance;  similar as above:\n",
    "\\begin{eqnarray}\n",
    " Var(X)&=&E X^2 - \\mu^2= M_X''(0)-\\left(\\lambda\\right)^2\\\\\n",
    "  &=& \\left.\\left[\\lambda e^te^{\\lambda(e^t-1)}+(\\lambda e^t)^2e^{\\lambda(e^t-1)}\\right]\\right|_{t=0}-\\lambda^2\\\\\n",
    "  &=&\\lambda+\\lambda^2-\\lambda^2=\\lambda\n",
    "\\end{eqnarray}\n"
   ]
  },
  {
   "cell_type": "markdown",
   "metadata": {},
   "source": [
    "\\begin{array}{|c|c|c|c|c|}\n",
    "  \\hline\n",
    "  r.v. & \\text{Probability Density Function} & \\text{Mean} & \\text{Variance} & \\text{Moment Generating Function}\\\\\n",
    "  \\hline\n",
    "\\text{Uniform}&f_X(x)=\\frac{1}{\\beta-\\alpha}&\\frac{\\beta+\\alpha}{2}&\\frac{(\\beta-\\alpha)^2}{12}&\\frac{e^{\\beta t}-e^{\\alpha t}}{t(b-a)} \\\\\\hline  \n",
    "\\text{Exponential}&f_X(x)=\\lambda e^{-\\lambda x}&\\frac{1}{\\lambda}&\\frac{1}{\\lambda^2}&\\frac{\\lambda}{\\lambda-t} \\\\\\hline\n",
    "\\text{Gamma}&\\frac{\\lambda^nx^{n-1}e^{-\\lambda x}}{\\Gamma(n)}&\\frac{n}{\\lambda}&\\frac{n}{\\lambda^2}&\\frac{\\lambda^n}{(\\lambda-t)^n} \\\\\\hline\n",
    "\\text{Normal}&\\frac{1}{\\sqrt{2\\pi}\\sigma}\\exp(-(x-\\mu)^2/2\\sigma^2)&\\mu&\\sigma^2&\\exp(\\sigma^2t^2/2+\\mu t) \\\\\\hline\n",
    "\\text{LogNormal}&\\frac{1}{\\sigma x\\sqrt{2\\pi}}e^{-(\\ln x-\\mu)^2/2\\sigma^2}&e^{\\mu+\\sigma^2/2}&(e^{\\sigma^2}-1)e^{2\\mu+\\sigma^2}&\\text{not defined}\\\\\\hline\n",
    "\\chi^2&\\frac{x^{n/2-1}e^{-x/2}}{2^{n/2}\\Gamma(n/2)}&n&2n&(1-2t)^{-n/2} \\\\\\hline\n",
    "t-\\text{student}&\\frac{\\Gamma((n+1)/2)}{\\sqrt{n\\pi}\\Gamma(n/2)}(1+x^2/n)^{-(n+1)/2}&0&\\frac{n}{n-2}&\\text{undefined} \\\\\\hline\n",
    "F&\\sqrt{\\frac{(d_1x)^{d_1}d_2^{d_2}}{(d_1x+d_2)^{d_1+d_2}}}\\left/{x\\beta(d_1/2,d_2/2)}\\right.&d_2/(d_2-2)&\\frac{2d_2^2(d_1+d_2-2)}{d_1(d_2-2)^2(d_2-4)}&\\text{does not exist} \\\\\\hline\n",
    "\\end{array}\n"
   ]
  },
  {
   "cell_type": "markdown",
   "metadata": {},
   "source": [
    "Continuous Uniform, \n",
    "---\n",
    "1. pdf: $f_X(x)=\\frac{1}{\\beta-\\alpha}$ for $x\\in[\\alpha,\\beta]$;\n",
    "- Mean:\n",
    "\\begin{eqnarray}\n",
    "   EX&=&\\int_\\alpha^\\beta \\frac{x dx}{\\beta-\\alpha}=\\left.\\frac{x^2}{2(\\beta-\\alpha)}\\right|_{\\alpha}^\\beta=\\frac{\\beta^2-\\alpha^2}{2(\\beta-\\alpha)}=\\frac{\\beta+\\alpha}{2}\n",
    " \\end{eqnarray}  \n",
    "- Variance;\n",
    "\\begin{eqnarray}\n",
    " EX^2&=&\\int_\\alpha^\\beta \\frac{x^2 dx}{\\beta-\\alpha}=\\left.\\frac{x^3}{3(\\beta-\\alpha)}\\right|_{\\alpha}^\\beta=\\frac{\\beta^3-\\alpha^3}{3(\\beta-\\alpha)}=\\frac{\\beta^2+\\alpha\\beta+\\alpha^2}{3}\\\\\n",
    " Var(X)&=&E X^2 - \\mu^2=\\frac{\\beta^2+\\alpha\\beta+\\alpha^2}{3}-\\left(\\frac{\\beta+\\alpha}{2}\\right)^2=\\frac{(\\beta-\\alpha)^2}{12}\n",
    "\\end{eqnarray}\n",
    "- MGF:\n",
    "\\begin{eqnarray}\n",
    "   E e^{tX}&=&\\int_\\alpha^\\beta \\frac{e^{tx} dx}{\\beta-\\alpha}=\\left.\\frac{e^{tx}}{t(\\beta-\\alpha)}\\right|_\\alpha^\\beta=\\frac{e^{\\beta t}-e^{\\alpha t}}{t(b-a)} \\\\\n",
    "\\end{eqnarray}"
   ]
  },
  {
   "cell_type": "markdown",
   "metadata": {},
   "source": [
    "Exponential, \n",
    "---\n",
    "1. pdf: $f_X(x)=\\lambda e^{-\\lambda x}$ for $x\\in[0,\\infty)$;\n",
    "- Mean:\n",
    "\\begin{eqnarray}\n",
    "   EX&=&\\int_0^\\infty\\lambda xe^{-\\lambda x} dx=\\int_0^\\infty\\lambda xe^{-\\lambda x} d(\\lambda x)\\cdot\\frac{1}{\\lambda}=\\Gamma(2)\\cdot\\frac{1}{\\lambda}=\\frac{1}{\\lambda}\n",
    " \\end{eqnarray} \n",
    " Here, $\\Gamma(n)=\\int_0^\\infty x^{n-1}e^{-x}dx=(n-1)!$.\n",
    "- Variance;\n",
    "\\begin{eqnarray}\n",
    " EX^2&=&\\int_0^\\infty\\lambda x^2e^{-\\lambda x} dx=\\int_0^\\infty(\\lambda x)^2e^{-\\lambda x} d(\\lambda x)\\cdot\\frac{1}{\\lambda^2}=\\Gamma(3)\\cdot\\frac{1}{\\lambda^2}=\\frac{2}{\\lambda^2}\\\\\n",
    " Var(X)&=&E X^2 - \\mu^2=\\frac{2}{\\lambda^2}-\\left(\\frac{1}{\\lambda}\\right)^2=\\frac{1}{\\lambda^2}\n",
    "\\end{eqnarray}\n",
    "- MGF:\n",
    "\\begin{eqnarray}\n",
    "   E e^{tX}&=&\\int_0^\\infty e^{tx}\\cdot\\lambda e^{-\\lambda x} dx=\n",
    "   \\frac{\\lambda}{\\lambda-t}\\int_0^\\infty ({\\lambda-t}) e^{-(\\lambda-t) x} dx\n",
    "   =\\frac{\\lambda}{\\lambda-t} \\\\\n",
    "\\end{eqnarray}"
   ]
  },
  {
   "cell_type": "markdown",
   "metadata": {},
   "source": [
    "Gamma$(n,\\lambda)$, \n",
    "---\n",
    "1. pdf: $f_X(x)=\\frac{\\lambda^nx^{n-1}e^{-\\lambda x}}{\\Gamma(n)}$ for $x\\in[0,\\infty)$;\n",
    "- Mean:\n",
    "\\begin{eqnarray}\n",
    "   EX&=&\\int_0^\\infty x\\cdot\\frac{\\lambda^nx^{n-1}e^{-\\lambda x}}{\\Gamma(n)} dx=\\int_0^\\infty(\\lambda x)^ne^{-\\lambda x} d(\\lambda x)\\cdot\\frac{1}{\\lambda\\Gamma(n)}=\\Gamma(n+1)\\cdot\\frac{1}{\\Gamma(n)\\lambda}=\\frac{n}{\\lambda}\n",
    " \\end{eqnarray} \n",
    " Here, $\\Gamma(n)=\\int_0^\\infty x^{n-1}e^{-x}dx=(n-1)!$.\n",
    "- Variance;\n",
    "\\begin{eqnarray}\n",
    " EX^2&=&\\int_0^\\infty x^2\\cdot\\frac{\\lambda^nx^{n-1}e^{-\\lambda x}}{\\Gamma(n)} dx=\\int_0^\\infty(\\lambda x)^{n+1}e^{-\\lambda x} d(\\lambda x)\\cdot\\frac{1}{\\lambda^2\\Gamma(n)}=\\Gamma(n+2)\\cdot\\frac{1}{\\Gamma(n)\\lambda^2}=\\frac{n(n+1)}{\\lambda^2}\\\\\n",
    " Var(X)&=&E X^2 - \\mu^2=\\frac{n(n+1)}{\\lambda^2}-\\frac{n^2}{\\lambda^2}=\\frac{n}{\\lambda^2}\n",
    "\\end{eqnarray}\n",
    "- MGF:\n",
    "\\begin{eqnarray}\n",
    "   E e^{tX}&=&\\int_0^\\infty e^{tx}\\cdot\\frac{\\lambda^nx^{n-1}e^{-\\lambda x}}{\\Gamma(n)} dx=\n",
    "   \\left(\\frac{\\lambda}{\\lambda-t}\\right)^n\\int_0^\\infty \\frac{({\\lambda-t})^nx^{n-1} e^{-(\\lambda-t) x}}{\\Gamma(n)} dx\n",
    "   =\\left(\\frac{\\lambda}{\\lambda-t}\\right)^n \\\\\n",
    "\\end{eqnarray}"
   ]
  },
  {
   "cell_type": "markdown",
   "metadata": {},
   "source": [
    "$\\chi^2(n)$, \n",
    "---\n",
    "$\\chi^2(n)$ is Gamma with $(n,\\lambda)\\Rightarrow(n/2,1/2)$"
   ]
  },
  {
   "cell_type": "markdown",
   "metadata": {},
   "source": [
    "Normal, $N(\\mu,\\sigma^2)$, \n",
    "---\n",
    "1. Consider $Z\\sim N(0,1)$, standard normal disttribution with pdf: $f_Z(z)=\\frac{1}{\\sqrt{2\\pi}}\\exp(-(z^2/2))$ for $z\\in\\mathbb{R}$;\n",
    "- Mean:\n",
    "\\begin{eqnarray}\n",
    "   E Z&=&\\int_{-\\infty}^\\infty \\frac{z}{\\sqrt{2\\pi}}\\exp(-z^2/2) dz=0\n",
    " \\end{eqnarray} \n",
    " since integrand is odd over $\\mathbb{R}$. And $EZ=0$\n",
    "- MGF:\n",
    "\\begin{eqnarray}\n",
    "   E e^{tZ}&=&\\int_{-\\infty}^\\infty \\frac{e^{tz}}{\\sqrt{2\\pi}}\\exp(-z^2/2) dz\\\\\n",
    "   &=&\\int_{-\\infty}^\\infty \\frac{1}{\\sqrt{2\\pi}}\\exp\\left(-\\left[(z^2-2zt+t^2)-t^2\\right]/2\\right) dz\\\\\n",
    "   &=&e^{t^2/2}\\cdot\\int_{-\\infty}^\\infty \\frac{1}{\\sqrt{2\\pi}}\\exp(-(z-t)^2/2) dz \\\\\n",
    "   &=& e^{t^2/2}\\cdot\\int_{-\\infty}^\\infty \\frac{1}{\\sqrt{2\\pi}}\\exp(-z^2/2) dz\\quad(\\text{by shift, i.e }z\\to z-t)\\\\\n",
    "  &=& e^{t^2/2}\\cdot \\frac{1}{\\sqrt{2\\pi}}\\cdot \\sqrt{2\\pi}=e^{-t^2/2}\n",
    "\\end{eqnarray}\n",
    "Here, use the fact $\\int_{-\\infty}^{\\infty}\\frac{e^{-z^2/a}}{\\sqrt{2\\pi}}dz=\\sqrt{a}$.\n",
    "- Variance;\n",
    "\\begin{eqnarray}\n",
    " EZ^2&=&M''(0)=\\left(t\\exp(t^2/2)\\right)'(0)\\\\\n",
    "     &=& \\left(\\exp(-t^2/2)+t^2\\exp(-t^2/2))\\right)_{t=0}=1\n",
    "\\end{eqnarray}\n",
    "- $X=\\mu+\\sigma Z\\sim N(\\mu,\\sigma^2)$, since \n",
    "  \\begin{eqnarray}\n",
    "  F_X(X<x)&=&F(\\mu+\\sigma Z<x)=F_Z(Z<\\frac{x-\\mu}{\\sigma})\\\\\n",
    "     &=& \\int_{-\\infty}^{\\frac{x-\\mu}{\\sigma}}\\frac{1}{\\sqrt{2\\pi}}e^{-z^2/2}dz\\\\\n",
    "  \\Rightarrow f_X(x)&=&F_X'(x)= \\frac{1}{\\sqrt{2\\pi}\\sigma}e^{-(x-\\mu)^2/(2\\sigma^2)}  \n",
    "  \\end{eqnarray}\n",
    "  - $E X=E(\\mu+\\sigma Z)=\\mu$,\n",
    "  - $Var(X)=Var(\\mu+\\sigma Z)=\\sigma^2Var(Z^2)=\\sigma^2$\n",
    "  - mgf of $X$ is\n",
    "    $$ MGF_X=Ee^{tX}=Ee^{t\\mu+t\\sigma Z}=e^{t\\mu}\\cdot e^{\\sigma^2 t^2/2}= e^{\\mu t+\\sigma^2 t^2/2}$$"
   ]
  },
  {
   "cell_type": "markdown",
   "metadata": {},
   "source": [
    "Normal, $N(\\mu,\\sigma^2)$, \n",
    "---\n",
    "1. pdf: $f_X(x)=\\frac{1}{\\sqrt{2\\pi}\\sigma}\\exp(-(x-\\mu)^2/2\\sigma^2)$ for $x\\in\\mathbb{R}$;\n",
    "- Mean:\n",
    "\\begin{eqnarray}\n",
    "   E(X-\\mu)&=&\\int_{-\\infty}^\\infty \\frac{(x-\\mu)}{\\sqrt{2\\pi}\\sigma}\\exp(-(x-\\mu)^2/2\\sigma^2) dx\\\\\n",
    "   &=&\\int_{-\\infty}^\\infty\\frac{(x)}{\\sqrt{2\\pi}\\sigma}\\exp(-(x)^2/2\\sigma^2)dx\n",
    "   =0\n",
    " \\end{eqnarray} \n",
    " since integrand is odd over $\\mathbb{R}$. And $EX=\\mu$\n",
    "- MGF:\n",
    "\\begin{eqnarray}\n",
    "   E e^{tX}&=&\\int_{-\\infty}^\\infty \\frac{e^{tx}}{\\sqrt{2\\pi}\\sigma}\\exp(-(x-\\mu)^2/2\\sigma^2) dx\\\\\n",
    "   &=&\\int_{-\\infty}^\\infty \\frac{1}{\\sqrt{2\\pi}\\sigma}\\exp\\left(\\left[x^2-2(\\mu+\\sigma^2t)x+(\\mu+\\sigma^2t)^2)+((\\mu+\\sigma^2t)^2-\\mu^2)\\right]/(2\\sigma^2)\\right) dx\\\\\n",
    "   &=&\\int_{-\\infty}^\\infty \\frac{1}{\\sqrt{2\\pi}\\sigma}\\exp((x-(\\mu+\\sigma^2t))^2/(2\\sigma^2))\\cdot\\exp((\\mu+\\sigma^2t)^2-\\mu^2)/(2\\sigma^2)) dx \\\\\n",
    "   &=& 1\\cdot\\exp((\\mu+\\sigma^2t)^2-\\mu^2)/(2\\sigma^2))=\\exp(\\mu t+\\sigma^2 t^2/2)\n",
    "\\end{eqnarray} \n",
    "- Variance;\n",
    "\\begin{eqnarray}\n",
    " EX^2&=&M''(0)=\\left((\\mu+\\sigma^2t)\\exp(\\mu t+\\sigma^2 t^2/2)\\right)'(0)\\\\\n",
    "     &=& \\left(\\sigma^2\\exp(\\mu t+\\sigma^2 t^2/2)+(\\mu+\\sigma^2t)^2\\exp(\\mu t+\\sigma^2 t^2/2)\\right)_{t=0}=\\sigma^2+\\mu^2\\\\\n",
    " Var(X)&=&E X^2 - \\mu^2=\\sigma^2+\\mu^2- \\mu^2=\\sigma^2\n",
    "\\end{eqnarray}\n"
   ]
  },
  {
   "cell_type": "markdown",
   "metadata": {},
   "source": [
    "LogNormal, $(\\mu,\\sigma^2)$, \n",
    "---\n",
    "1. pdf: $f_Y(y)=\\frac{1}{\\sigma y\\sqrt{2\\pi}}e^{-(\\ln y-\\mu)^2/2\\sigma^2}$ for $x\\in(0,\\infty)$;\n",
    "- Mean:<br>\n",
    "Suppose that $X$ is normal, with MGF $Ee^{tX}=\\exp(\\sigma^2t^2/2+\\mu t)$; $Y=\\exp(X)$ is LogNormal($\\mu,\\sigma^2)$\n",
    "\\begin{eqnarray}\n",
    "   E(Y)&=&Ee^{X}=\\left.\\exp(\\sigma^2t^2/2+\\mu t) \\right|_{t=1}\\\\\n",
    "   &=&e^{\\mu+\\sigma^2/2}\n",
    " \\end{eqnarray} \n",
    "- Variance;\n",
    "\\begin{eqnarray}\n",
    " EY^2&=&Ee^{2X}=\\left.\\exp(\\sigma^2t^2/2+\\mu t) \\right|_{t=2}\\\\\n",
    "     &=& e^{2\\mu+2\\sigma^2}\\\\\n",
    " Var(Y)&=&E Y^2 - (EY)^2=e^{2\\mu+2\\sigma^2}- (e^{\\mu+\\sigma^2/2})^2=(e^{\\sigma^2}-1)e^{2\\mu+\\sigma^2}\n",
    "\\end{eqnarray}\n",
    "- MGF:\n",
    "Not defines\n",
    "\n",
    "\n"
   ]
  },
  {
   "cell_type": "markdown",
   "metadata": {},
   "source": [
    "Student, $T(n)$, \n",
    "---\n",
    "1. pdf: $f_X(x)=\\frac{\\Gamma((n+1)/2}{\\sqrt{n\\pi}\\Gamma(n/2)}(1+x^2/n)^{-(n+1)/2}$ for $x\\in\\mathbb{R}$;\n",
    "- Mean:<br>\n",
    "\\begin{eqnarray}\n",
    "   E(X)&=&\\int_{-\\infty}^{\\infty}x\\cdot\\frac{\\Gamma((n+1)/2)}{\\sqrt{n\\pi}\\Gamma(n/2)}(1+x^2/n)^{-(n+1)/2}dx=0\n",
    "\\end{eqnarray}\n",
    "since $\\frac{x}{(1+x^2/n)^{-(n+1)/2}}$ is odd over $(-\\infty,\\infty)$.\n",
    "- Variance;\n",
    "Let $c=\\frac{\\Gamma((n+1)/2)}{\\sqrt{n\\pi}\\Gamma(n/2)}$,\n",
    "\\begin{eqnarray}\n",
    " Var(x)&=&EX^2=\\int_{-\\infty}^{\\infty}x^2\\cdot\\frac{\\Gamma((n+1)/2)}{\\sqrt{n\\pi}\\Gamma(n/2)}(1+x^2/n)^{-(n+1)/2}dx\\\\\n",
    "     &=& c\\dot\\int_{-\\infty}^{\\infty}x^2(1+x^2/n)^{-(n+1)/2}dx\\\\\n",
    "     &=&2c\\dot\\int_{0}^{\\infty}x^2(1+x^2/n)^{-(n+1)/2}dx, \\text{ since even,}\\\\\n",
    "     &=&2c\\int_{0}^{\\infty}nt(1+t)^{-n/2-1/2}\\frac{\\sqrt n}{2}\\frac{1}{\\sqrt t}dt, \\text{ by change of variable }t=x^2/n,\\\\\n",
    "     &=&cn^{3/2}\\int_0^\\infty t^{3/2-1}{(1+t)}^{-3/2-(n/2-1)}dt=cn^{3/2}\\beta(3/2,n/2-1)\\\\\n",
    "     &=&n^{3/2}\\frac{{\\Gamma((n+1)/2)}}{\\sqrt{n\\pi}\\Gamma(n/2)}\\frac{\\Gamma(3/2)\\Gamma(n/2-1)}{\\Gamma((n+1)/2)}\\\\\n",
    "     &=&n^{3/2}\\frac{\\frac{1}{2}\\Gamma(1/2)\\Gamma(n/2-1)}{\\sqrt{n\\pi}(n/2-1)\\Gamma(n/2-1)}=\\frac{n}{n-2}\n",
    "\\end{eqnarray}\n",
    "where \n",
    "$$\\beta(a,b)=\\int_0^\\infty t^{a-1}(1+t)^{-a-b}dt=\\frac{\\Gamma(a)\\Gamma(b)}{\\Gamma(a+b)},\\Gamma(a+1)=a\\Gamma(a),\\Gamma(1/2)=\\sqrt{\\pi}$$\n",
    "- MGF:-\n",
    "Not defines\n",
    "\n",
    "\n"
   ]
  },
  {
   "cell_type": "code",
   "execution_count": null,
   "metadata": {},
   "outputs": [],
   "source": []
  },
  {
   "cell_type": "markdown",
   "metadata": {},
   "source": [
    "Relations between r.v.'s\n",
    "---\n",
    "U-uniform $\\leftrightarrow$ Binomial($n,p$)\n",
    "---\n",
    "- let $U\\sim$ U(0,1), and difine \n",
    "     $$ X=\\left\\{ \\begin{array}{l}\n",
    "       1 \\text{, if } 0\\le U <p ,\\\\\n",
    "       0, \\text{, if } p\\le U \\le 1\n",
    "     \\end{array} \\right.$$\n",
    "    Then $X$ is Bernoulli($p$) since \n",
    "     $$ X=\\left\\{ \\begin{array}{l}\n",
    "       1 \\text{, with probability } p ,\\\\\n",
    "       0, \\text{ with probability } 1-p\n",
    "     \\end{array} \\right.$$\n",
    "    and pmf is \n",
    "    $$Ee^{tX}=e^{t\\cdot1}p+ e^{t\\cdot0}(1-p)=1-p+pe^t$$\n",
    "    Sum of i.i.d. of $X$, $Y=\\sum\\limits^n X_i$ where $X_i\\sim X$ is Binomial($n,p$):   \\begin{eqnarray}\n",
    "    Ee^{tY}&=&E e^{\\sum(tX_i)}\\\\\n",
    "       &=&\\prod^n Ee^{tX_i}\\\\\n",
    "       &=&(1-p+pe^t)^n\n",
    "\\end{eqnarray}\n",
    "i.e. $Y$ is binonial distributed.\n",
    "\n",
    "- D-uniform, \n",
    "  $$ U=\\left\\{ \\begin{array}{l}\n",
    "       1 \\text{ with probability }1/2,\\\\\n",
    "       0, \\text{ with probability } 1/2\n",
    "     \\end{array} \\right.$$\n",
    "  U is also Bernulli(1/2). Let $\\{U_i\\}$ be i.i.d $\\sim U$. As same reason, $Y=\\sum^n U_i$ is Binomial($n,1/2$).    "
   ]
  },
  {
   "cell_type": "markdown",
   "metadata": {},
   "source": [
    "C-unif $\\leftrightarrow$ Poisson($\\lambda$)\n",
    "---\n",
    "  Suppose that $U \\sim U(0,1)$; then $X=-\\log U$ is exponential($\\lambda=1$):\n",
    "\n",
    "\\begin{eqnarray*}\n",
    "   P(X\\le x) &=& P(-\\log U\\le x)=P(U \\ge e^{-x})\\\\\n",
    "             &=& 1-e^{-x}\\\\\n",
    "     \\Rightarrow p_X(x) &=&  P'(X\\le x) \\\\ \n",
    "             &=& e^{-x}\n",
    "\\end{eqnarray*}\n",
    "i.e. $X$ is exponential(1) or int-arrivaltime of a Poisson processes having rate $\\lambda=1$. \n",
    "  - sum of $X_i$, $X=\\sum^n X_i$, where $X_i\\sim X=Exp(1)$ is Gamma$(n,1)=\\Gamma(n,1)$:\n",
    "  \\begin{eqnarray}\n",
    "    E e^{tX}_i&=&\\int_0^\\infty e^{tx}e^{-x} dx=\\int_0^\\infty e^{-(1-t)x} dx=\\frac{1}{1-t}\\\\\n",
    "    Ee^{tX}&=&E e^{\\sum(tX_i)}\\\\\n",
    "       &=&\\prod^n Ee^{tX_i}\\\\\n",
    "       &=&(1-t)^{-n}\n",
    "\\end{eqnarray} \n",
    "i.e. pdf of $X, f_X(x)=x^{n-1}e^{-x}/{(n-1)}!, x\\ge0$\n",
    "  - Consider the Number of enents,\n",
    "\\begin{eqnarray}\n",
    "  N(1)=N&=&\\max\\left\\{ n:\\sum_n X_i<1 \\right\\}\\\\\n",
    "      &=& \\frac{1^{n-1}e^{-1}}{n!}\\\\\n",
    "  \\Rightarrow  N(\\lambda)&=&\\max\\left\\{ n:\\sum_n X_i<\\lambda \\right\\}\\\\ \n",
    "      &=& \\frac{\\lambda^{n-1}e^{-\\lambda}}{n!}\n",
    "\\end{eqnarray}\n",
    "\n",
    "Thus $Y=N(\\lambda)-1=0,1,2,3,\\cdots,$ is Poisson distributed with $\\lambda$.\n",
    "\n"
   ]
  },
  {
   "cell_type": "markdown",
   "metadata": {},
   "source": [
    "Binomial($n,p$) $\\leftrightarrow$ Poisson($\\lambda$)\n",
    "---\n",
    "- $np\\sim \\lambda$, while $n\\to\\infty$\n",
    "- Consider $X\\sim$ Binomial($n,p$)\n",
    "\\begin{eqnarray*}\n",
    "   Ee^{tX} &=& (1-p+pe^t)^n=\\left(1+\\frac{np(e^t-1)}{n}\\right)^n\\\\\n",
    "            (\\text{ as } n\\to\\infty) &\\Rightarrow& e^{\\lambda(e^t-1)}\n",
    "\\end{eqnarray*}\n",
    "by the Euler limit result:\n",
    "$$\\lim_{n\\to\\infty}\\left(1+\\frac{a}{n}\\right)^n=e^a$$\n",
    "and this $X$ is  Poisson($\\lambda$) while $n\\to\\infty$."
   ]
  },
  {
   "cell_type": "markdown",
   "metadata": {},
   "source": [
    "Geometric($p$) $\\leftrightarrow$ NegBin($n,p$)\n",
    "---\n",
    "- $X\\sim Geometric(p)$, pmf = $ p(1-p)^k$, $k=0,1,2,\\cdots$;\n",
    "- $Y\\sim NB(n,p)$, pmf= $C^{n+k-1}_k p^n(1-p)^k$, $k=0,1,2,\\cdots$.\n",
    "\n",
    "Obviously, $NB(1,p)=Geometric(p)$, i.e. $n=1$."
   ]
  },
  {
   "cell_type": "markdown",
   "metadata": {},
   "source": [
    "Geo($p$) $\\leftrightarrow$ Exponential($\\lambda$)\n",
    "---\n",
    "\n",
    "- let $T\\sim Exp(\\lambda)$, pdf, $f_T(t)=\\lambda e^{-\\lambda t}$\n",
    "\n",
    "\\begin{eqnarray*}\n",
    "   P(T\\ge t) &=& \\int_t^\\infty \\lambda e^{-\\lambda s}ds= e^{-\\lambda t}\n",
    "\\end{eqnarray*}\n",
    "\n",
    "- $X\\sim$ with pmf \n",
    "$$P(X=n)=p(1-p)^{n-1}, n=1,2,3,\\cdots$$\n",
    "\n",
    "\\begin{eqnarray*}\n",
    "   P(X>n) &=& \\sum_{k=n+1}^\\infty p(1-p)^{k-1}\\\\\n",
    "      &=& p(1-p)^n+p(1-p)^{n+1}+p(1-p)^{n+2}+\\cdots\\\\\n",
    "      &=&p\\frac{(1-p)^n}{1-(1-p)}=(1-p)^n\n",
    "\\end{eqnarray*}\n",
    ", i.e. for Poisson Process, with the  rate $\\lambda t$.\n",
    "\n",
    "Let $X_\\tau\\sim Geo(p=\\lambda\\tau)$, where $\\tau$ is a short time duration, then consider $X_\\tau\\tau$:\n",
    "\\begin{eqnarray*}\n",
    "   P(X_\\tau\\tau>t) &=& P(X_\\tau>\\frac{t}{\\tau})\\\\\n",
    "    &=&(1-\\lambda\\tau)^{[\\frac{t}{\\tau}]}\\to e^{-\\lambda t}\n",
    "\\end{eqnarray*}\n",
    "i.e. $X_\\tau\\tau$ is approximated Exp($\\lambda$) as $\\tau$ is small."
   ]
  },
  {
   "cell_type": "code",
   "execution_count": null,
   "metadata": {},
   "outputs": [],
   "source": []
  },
  {
   "cell_type": "markdown",
   "metadata": {},
   "source": [
    " Poisson($\\lambda$) $\\leftrightarrow$ Exponential($\\lambda$)\n",
    "---\n",
    "- Let $X\\sim$ Poisson($\\lambda$), pmf\n",
    "  $$P(X=k)=\\frac{e^{-\\lambda}(\\lambda)^k}{k!}, k=0,1,2,3,\\cdots$$\n",
    "- let $T\\sim Exp(\\lambda)$, pdf, $f_T(t)=\\lambda e^{-\\lambda t}$\n",
    "\n",
    "\\begin{eqnarray*}\n",
    "   P(T\\ge t) &=& \\int_t^\\infty \\lambda e^{-\\lambda s}ds= e^{-\\lambda t}\n",
    "\\end{eqnarray*}\n",
    "The event occur at more than $t$ at the rate $\\lambda$; in other words, there is no event, $k=0$:\n",
    "\\begin{eqnarray*}\n",
    "   P(X=0) &=& P(T\\ge t) =e^{-\\lambda t}=\\frac{e^{-\\lambda t} (-\\lambda t)^0}{0!}\n",
    "\\end{eqnarray*}\n",
    ", i.e. for Poisson Process, with the  rate $\\lambda t$.\n",
    "\n"
   ]
  },
  {
   "cell_type": "markdown",
   "metadata": {},
   "source": [
    " Exponential($\\lambda$) $\\leftrightarrow$  Gamma($n,\\lambda$)\n",
    "---\n",
    "- MGF of Let $X\\sim$ Exponential($\\lambda$) \n",
    "  $$E e^{tX}=\\frac{\\lambda}{\\lambda-t}$$\n",
    "- Consider Y, sum of i.i.d of $\\{X_i\\}$ where $X_i\\sim X$, MGF of $Y$ is\n",
    "\\begin{eqnarray*}\n",
    "   Ee^{tY} &=& Ee^{\\sum^ntX_i}\\\\\n",
    "     &=&\\prod^nE e^{tX_i}=\\left(\\frac{\\lambda}{\\lambda-t}\\right)^n\n",
    "\\end{eqnarray*}\n",
    "i.e. $ Y\\sim $ Gamma($n,\\lambda$)"
   ]
  },
  {
   "cell_type": "markdown",
   "metadata": {},
   "source": [
    " Poisson($\\lambda$) $\\leftrightarrow$ Gamma(n,$\\lambda$)\n",
    "---\n",
    "- Let $X\\sim$ Poisson($\\lambda t$), pmf\n",
    "  $$P(X=k)=\\frac{e^{-\\lambda t}(\\lambda t)^k}{k!}, k=0,1,2,3,\\cdots$$\n",
    "- Let $T$ be the time until $k$ events occur\n",
    "\n",
    "\\begin{eqnarray*}\n",
    "   F_T(t)=P(T\\le t) &=& 1-P(T> t)=1-P(X<k)=1-P(X\\le k-1)\\\\\n",
    "       &=&1-\\sum^{k-1}_{x=0}\\frac{(\\lambda t)^x e^{-\\lambda t}}{x!}\\\\\n",
    "   \\Rightarrow f_T(t)&=&\\lambda e^{-\\lambda t}\\sum^{k-1}_{x=0}\\frac{(\\lambda t)^x }{x!}\n",
    "   - e^{-\\lambda t}\\sum^{k-1}_{x=0}\\frac{x\\lambda(\\lambda t)^{x-1}}{x!}\\\\\n",
    "   &=&\\lambda e^{-\\lambda t}\\sum^{k-1}_{x=0}\\frac{(\\lambda t)^x }{x!}-e^{-\\lambda t}\\sum^{k-1}_{x=1}\\frac{x\\lambda(\\lambda t)^{x-1}}{x!}\\\\\n",
    "   &=&\\lambda e^{-\\lambda t}\\sum^{k-1}_{x=0}\\frac{(\\lambda t)^x }{x!}-e^{-\\lambda t}\\sum^{k-1}_{x=1}\\frac{\\lambda(\\lambda t)^{x-1}}{(x-1)!}\\\\\n",
    "   &=&\\lambda e^{-\\lambda t}\\sum^{k-1}_{x=0}\\frac{(\\lambda t)^x }{x!}-e^{-\\lambda t}\\sum^{k-2}_{x=0}\\frac{\\lambda(\\lambda t)^{x}}{(x)!}\\\\\n",
    "   &=& \\frac{\\lambda^kt^{k-1}e^{-\\lambda t}}{(k-1)!}=\\frac{\\lambda^kt^{k-1}e^{-\\lambda t}}{\\Gamma(k)}\n",
    "\\end{eqnarray*}\n",
    "This concludes $T$ is $\\Gamma(n,\\lambda)$.\n"
   ]
  },
  {
   "cell_type": "markdown",
   "metadata": {},
   "source": [
    "Normal $N(\\mu,\\sigma^2)$ $\\leftrightarrow$  LogNormal $LN(\\mu,\\sigma^2)$\n",
    "---\n",
    "- $X\\sim N(\\mu,\\sigma^2)$  \n",
    "Consider $Y\\sim \\exp(X)$:\n",
    "\n",
    "\\begin{eqnarray*}\n",
    "   P(Y\\le y) &=& P(\\exp X\\le y)= P(X\\le\\log y)\\\\\n",
    "     &=&\\int_{-\\infty}^{\\log y}\\frac{1}{\\sqrt{2\\pi}\\sigma}\\exp\\left(-\\frac{(x-\\mu)^2}{2\\sigma^2}\\right)dx\\\\\n",
    "   f_Y(y)&=&  \\left(P(Y\\le y)\\right)'\\\\\n",
    "         &=& \\frac{1}{y\\sigma\\sqrt{2\\pi}}\\exp\\left(-\\frac{(\\log y-\\mu)^2}{2\\sigma^2}\\right)\n",
    "\\end{eqnarray*}\n",
    "i.e. $ Y\\sim LN(\\mu,\\sigma^2)$"
   ]
  },
  {
   "cell_type": "code",
   "execution_count": null,
   "metadata": {},
   "outputs": [],
   "source": []
  },
  {
   "cell_type": "code",
   "execution_count": null,
   "metadata": {},
   "outputs": [],
   "source": []
  },
  {
   "cell_type": "markdown",
   "metadata": {},
   "source": [
    "Homework 2\n",
    "---\n",
    "\n",
    "- $Z^2\\sim \\chi^2(1)$: Suppose that $Z=N(0,1)$ and its MGF is $e^{-t^2/2}$, then\n",
    "$$ E e^{tZ^2}=\\int_{-\\infty}^{\\infty}\\frac{1}{\\sqrt{2\\pi}}\\exp(-tz^2-z^2/2)dz\n",
    "       =\\int_{-\\infty}^{\\infty}\\frac{1}{\\sqrt{2\\pi}}\\exp(-\\frac{z^2}{2}(1-2t))dz=\\frac{1}{\\sqrt{1-2t}}$$\n",
    "Since\n",
    "$$\\int_{-\\infty}^{\\infty}\\frac{1}{\\sqrt{2\\pi}}\\exp(-\\frac{z^2}{2})dz=1$$\n",
    "and\n",
    "$$\\int_{-\\infty}^{\\infty}\\frac{1}{\\sqrt{2\\pi}}\\exp(-\\frac{az^2}{2})dz=\\frac{1}{\\sqrt a}$$\n",
    "This is MGF of $\\chi^2(1)$.\n",
    "- sum of $n$ i.i.d. of $\\chi^2(1)$ is distributed as $\\chi^2(n)$:\n",
    "Suppose that $X=\\sum_{i}^nX_i$ where $\\{X_i\\}$ i.i.d of $\\chi^2(1)$:\n",
    "$$E e^{tX}=Ee^{\\sum tX_i}=\\prod Ee^{tX_i}=\\left(\\frac{1}{1-2t}\\right)^n$$\n",
    "- For independent $Z$, $Y=\\chi^2(n)$, the $Z/\\sqrt{Y/n}$ is $t$ r.v. with degree $n$:\n",
    "Consider the jointly pdf of  $(Z, Y)$\n",
    "  into $(T, V) $:\n",
    "\n",
    "$$  f_{Z,Y}(z,y)=\\frac{1}{\\sqrt{2 \\pi}} e^{- \\frac{z^2}{2}}\\cdot \n",
    "     \\frac{y^{n / 2 - 1} e^{- y / 2}}{\\Gamma (n / 2) 2^{n /2}} $$\n",
    "  where $-\\infty<z<\\infty,0\\le y<\\infty$.\n",
    "\n",
    "Now let $ t = \\frac{z}{\\sqrt{\\frac{y}{n}}} \\text{ and } v = y $; thus $y=v, z=t \\sqrt{\\frac{v}{n}}$ with Jacobian:\n",
    "$$\n",
    "\\left|\\frac{\\partial(z,y)}{\\partial(t,v)}\\right|=\n",
    "\\begin{pmatrix}\n",
    "  \\sqrt{\\frac{v}{n}}&\\frac{t}{2\\sqrt{nv}}\\\\\n",
    "  0&1\n",
    "  \\end{pmatrix}\n",
    "$$\n",
    "\n",
    "Moreover, we have\n",
    "\n",
    "\\begin{eqnarray*}\n",
    "   f_T(t)&=& \\int f_{T,V}(x(t,v),y(t,v))\\left|\\frac{\\partial(x,y)}{\\partial(t,v)}\\right|dv\\cr\\\\\n",
    "    &=&\\int^{\\infty}_0 \\frac{1}{\\sqrt{2 \\pi}} e^{- \\frac{(t\\sqrt{v/n})^2}{2}}\n",
    "         \\frac{v^{n / 2 - 1} e^{- v / 2}}{\\Gamma (n / 2) 2^{n /2}} \\sqrt{\\frac{v}{n}}dv\\\\\n",
    "    &=&  \\frac{1}{\\sqrt{2 \\pi n}\\Gamma (n / 2) 2^{ n/ 2} } \\int^{\\infty}_0\n",
    "    v^{\\frac{n+1}{2}-1}e^{-v((1+t^2/n)/2)}dv \\\\\n",
    "    &=&  \\frac{1}{\\sqrt{2 \\pi n}\\Gamma (n / 2) 2^{ n/ 2} }\n",
    "        \\left( (1+t^2/n)/2\\right)^{-(n+1)/2}\n",
    "        \\int^{\\infty}_0w^{\\frac{n+1}{2}-1} e^{-w} dw\\\\\n",
    "    &=& \\frac{\\Gamma ((n+1)/ 2)}{\\sqrt{\\pi n}\\Gamma (n / 2) }\n",
    "        \\left( (1+t^2/n)\\right)^{-(n+1)/2}\\\\\n",
    "    & = & f_T (t) \\text{ where } - \\infty < t < \\infty\n",
    "  \\end{eqnarray*}\n",
    "\n",
    "where \n",
    "$$\\Gamma(n)=\\int_0^\\infty x^{n-1}e^{-x}dx=(n-1)!$$\n",
    "This proves $T$ is  $t$-distribution. \n",
    "\n"
   ]
  },
  {
   "cell_type": "code",
   "execution_count": null,
   "metadata": {},
   "outputs": [],
   "source": []
  },
  {
   "cell_type": "code",
   "execution_count": null,
   "metadata": {},
   "outputs": [],
   "source": []
  },
  {
   "cell_type": "code",
   "execution_count": null,
   "metadata": {},
   "outputs": [],
   "source": []
  }
 ],
 "metadata": {
  "kernelspec": {
   "display_name": "Python 3",
   "language": "python",
   "name": "python3"
  },
  "language_info": {
   "codemirror_mode": {
    "name": "ipython",
    "version": 3
   },
   "file_extension": ".py",
   "mimetype": "text/x-python",
   "name": "python",
   "nbconvert_exporter": "python",
   "pygments_lexer": "ipython3",
   "version": "3.6.9"
  }
 },
 "nbformat": 4,
 "nbformat_minor": 2
}
